Mica/Verifier/Specifications.lean
@@ -1,5 +1,4 @@
 import Mica.TinyML.Typed
-import Mica.TinyML.Erasure
 import Mica.TinyML.Typing
 import Mica.TinyML.WeakestPre
 import Mica.FOL.Printing
